extraction/extraction.v
@@ -20,21 +20,27 @@ Require DecidableClass Decidableplus.
 Require AST.
 Require Iteration.
 Require Floats.
-Require SelectLong.
-Require Selection.
-Require RTLgen.
-Require Inlining.
-Require ValueDomain.
-Require Tailcall.
-Require Allocation.
-Require Bounds.
 Require Ctypes.
 Require Csyntax.
-Require Ctyping.
-Require Clight.
-Require Compiler.
 Require Parser.
 Require Initializers.
+
+Require Import Tags Initializers Csem.
+
+Module I := Initializers NullTag NullPolicy.
+Import I.
+Import Cexec.
+Import Cstrategy.
+Import Ctyping.
+Import Csem.
+Import Csyntax.
+Import Cop.
+Import Deterministic.
+Import Behaviors.
+Import Smallstep.
+Import Events.
+Import Genv.
+Import Mem.
 
 (* Standard lib *)
 Require Import ExtrOcamlBasic.
@@ -57,7 +63,7 @@ Extraction Inline DecidableClass.Decidable_witness DecidableClass.decide
 Extraction Inline Wfsimpl.Fix Wfsimpl.Fixm.
 
 (* Memory - work around an extraction bug. *)
-Extraction NoInline Memory.Mem.valid_pointer.
+Extraction NoInline valid_pointer.
 
 (* Errors *)
 Extraction Inline Errors.bind Errors.bind2.
@@ -68,64 +74,6 @@ Extract Constant Iteration.GenIter.iterate =>
   "let rec iter f a =
      match f a with Coq_inl b -> Some b | Coq_inr a' -> iter f a'
    in iter".
-
-(* Selection *)
-
-Extract Constant Selection.compile_switch => "Switchaux.compile_switch".
-Extract Constant Selection.if_conversion_heuristic => "Selectionaux.if_conversion_heuristic".
-
-(* RTLgen *)
-Extract Constant RTLgen.more_likely => "RTLgenaux.more_likely".
-Extraction Inline RTLgen.ret RTLgen.error RTLgen.bind RTLgen.bind2.
-
-(* Inlining *)
-Extract Inlined Constant Inlining.should_inline => "Inliningaux.should_inline".
-Extract Inlined Constant Inlining.inlining_info => "Inliningaux.inlining_info".
-Extract Inlined Constant Inlining.inlining_analysis => "Inliningaux.inlining_analysis".
-Extraction Inline Inlining.ret Inlining.bind.
-
-(* Allocation *)
-Extract Constant Allocation.regalloc => "Regalloc.regalloc".
-
-(* Linearize *)
-Extract Constant Linearize.enumerate_aux => "Linearizeaux.enumerate_aux".
-
-(* SimplExpr *)
-Extract Constant SimplExpr.first_unused_ident => "Camlcoq.first_unused_ident".
-Extraction Inline SimplExpr.ret SimplExpr.error SimplExpr.bind SimplExpr.bind2.
-
-(* Compopts *)
-Extract Constant Compopts.optim_for_size =>
-  "fun _ -> !Clflags.option_Osize".
-Extract Constant Compopts.va_strict =>
-  "fun _ -> false".
-Extract Constant Compopts.propagate_float_constants =>
-  "fun _ -> !Clflags.option_ffloatconstprop >= 1".
-Extract Constant Compopts.generate_float_constants =>
-  "fun _ -> !Clflags.option_ffloatconstprop >= 2".
-Extract Constant Compopts.optim_tailcalls =>
-  "fun _ -> !Clflags.option_ftailcalls".
-Extract Constant Compopts.optim_constprop =>
-  "fun _ -> !Clflags.option_fconstprop".
-Extract Constant Compopts.optim_CSE =>
-  "fun _ -> !Clflags.option_fcse".
-Extract Constant Compopts.optim_redundancy =>
-  "fun _ -> !Clflags.option_fredundancy".
-Extract Constant Compopts.thumb =>
-  "fun _ -> !Clflags.option_mthumb".
-Extract Constant Compopts.debug =>
-  "fun _ -> !Clflags.option_g".
-
-(* Compiler *)
-Extract Constant Compiler.print_Clight => "PrintClight.print_if".
-Extract Constant Compiler.print_Cminor => "PrintCminor.print_if".
-Extract Constant Compiler.print_RTL => "PrintRTL.print_if".
-Extract Constant Compiler.print_LTL => "PrintLTL.print_if".
-Extract Constant Compiler.print_Mach => "PrintMach.print_if".
-Extract Constant Compiler.print => "fun (f: 'a -> unit) (x: 'a) -> f x; x".
-Extract Constant Compiler.time  => "Timing.time_coq".
-
-(*Extraction Inline Compiler.apply_total Compiler.apply_partial.*)
 
 (* Cabs *)
 Extract Constant Cabs.loc =>
@@ -139,8 +87,6 @@ Extract Constant Cabs.char_code => "int64".
 
 (* Processor-specific extraction directives *)
 
-Load extractionMachdep.
-
 (* Avoid name clashes *)
 Extraction Blacklist List String Int.
 
@@ -152,25 +98,15 @@ Set Extraction AccessOpaque.
 Cd "extraction".
 
 Separate Extraction
-   Compiler.transf_c_program Compiler.transf_cminor_program
    Cexec.do_initial_state Cexec.do_step Cexec.at_final_state
    Ctypes.merge_attributes Ctypes.remove_attributes Ctypes.build_composite_env
-   Initializers.transl_init Initializers.constval
+   transl_init constval
    Csyntax.Eindex Csyntax.Epreincr Csyntax.Eselection
    Ctyping.typecheck_program
    Ctyping.epostincr Ctyping.epostdecr Ctyping.epreincr Ctyping.epredecr
    Ctyping.eselection
    Ctypes.make_program
-   Clight.type_of_function
-   Conventions1.callee_save_type Conventions1.is_float_reg
-   Conventions1.int_caller_save_regs Conventions1.float_caller_save_regs
-   Conventions1.int_callee_save_regs Conventions1.float_callee_save_regs
-   Conventions1.dummy_int_reg Conventions1.dummy_float_reg
-   RTL.instr_defs RTL.instr_uses
-   Machregs.mregs_for_operation Machregs.mregs_for_builtin
-   Machregs.two_address_op Machregs.is_stack_reg
-   Machregs.destroyed_at_indirect_call
-   AST.signature_main
+   AST
    Floats.Float32.from_parsed Floats.Float.from_parsed
-   Globalenvs.Senv.invert_symbol
+   invert_symbol
    Parser.translation_unit_file.
